\section{Mathematical Logic}
\subsection*{Exercises}
\begin{questions}
    \item We work from the inner-most bracket outwards. We note $p$ is true, $q$ is false, and $r$ is true.
    \begin{itemize}
        \item $p \lor q$ is ``1 is a positive number \textbf{or} $-1 > 0$'', which is true since $p$ is true.
        \item $(p \lor q) \land r$ is ``(1 is a positive number or $-1 > 0$) \textbf{and} 1 is an odd number'', which is true since $p \lor q$ is true and 1 is, indeed, an odd number.
        \item $\lnot((p \lor q) \land r)$ is false, since $(p \lor q) \land r$ is true.
    \end{itemize}
    Hence the statement ``$\lnot((p \lor q) \land r)$ is false'' is a true statement.

    \item The truth table for $p \land \lnot q$ is given below.
    \begin{table}[H]
        \centering
        \begin{tabular}{|l|l||l|}
            \hline
            $\boldsymbol{p}$ & $\boldsymbol{q}$ & $\boldsymbol{p\land \lnot q}$ \\ \hline
            F & F & F \\ \hline
            F & T & F \\ \hline
            T & F & T \\ \hline
            T & T & F \\ \hline
        \end{tabular}
    \end{table}

    We will see that, in fact, this is the negation of $p \implies q$ later.

    \item \begin{partquestions}{\roman*}
        \item $r$: $n$ is a multiple of 5 if and only if the last digit of $n$ is 0 or 5.
        \item If $n$ is a multiple of 5, then its last digit necessarily has to be 5 or 0, hence $p \implies q$. If the last digit is 5 or 0, then the number $n$ is a multiple of 5, hence $q \implies p$. Therefore $p \iff q$.
    \end{partquestions}

    \item For brevity, let $r = p \implies \lnot q$ and $s = \lnot q \implies p$. So we want to show that $(\lnot p \iff q) \equiv r \land s$.
    \begin{table}[H]
        \centering
        \begin{tabular}{|l|l||l|l|l|l||l|l|}
            \hline
            $\boldsymbol{p}$ & $\boldsymbol{q}$ & $\boldsymbol{\lnot p}$ & $\boldsymbol{\lnot q}$ & $\boldsymbol{r}$ & $\boldsymbol{s}$ & $\boldsymbol{r \land s}$ & $\boldsymbol{\lnot p \iff q}$ \\ \hline
            F & F & T & T & T & F & F & F \\ \hline
            F & T & T & F & T & T & T & T \\ \hline
            T & F & F & T & T & T & T & T \\ \hline
            T & T & F & F & F & T & F & F \\ \hline
        \end{tabular}
    \end{table}

    From inspection, the truth tables of $\lnot p \iff q$ and $r \land s$ are the same, proving our required result.

    \item We work slowly.
    {
        \fontsize{8.5pt}{11pt}\selectfont
        \begin{align*}
            &((p \lor \lnot q) \land \lnot r) \lor ((p \lor \lnot q) \land (p \lor r) \land (p \lor \lnot r))\\
            &\equiv ((p \lor \lnot q) \land \lnot r) \lor ((p \lor \lnot q) \land ((p \lor r) \land (p \lor \lnot r))) & (\text{Associativity})\\
            &\equiv (p \lor \lnot q) \land (\lnot r \lor ((p \lor r) \land (p \lor \lnot r))) & (\text{Distributivity})\\
            &\equiv (p \lor \lnot q) \land (\lnot r \lor (p \lor (r \land \lnot r))) & (\text{Distributivity})\\
            &\equiv (p \lor \lnot q) \land (\lnot r \lor (p \lor \textbf{false}))\\
            &\equiv (p \lor \lnot q) \land (\lnot r \lor p)\\
            &\equiv (p \lor \lnot q) \land (p \lor \lnot r) & (\text{Commutativity})\\
            &\equiv p \lor (\lnot q \land \lnot r) & (\text{Distributivity})\\
            &\equiv p \lor \lnot(q \lor r) & (\text{De Morgan's Law})
        \end{align*}
    }

    \item $\left((n \in \mathbb{Z}) \land (n > 2)\right) \implies \left(\exists a, b \in \mathbb{Z} \text{ s.t. } a^3 + b^4 = n^5\right)$

    \item \begin{partquestions}{\roman*}
        \item Let
        \begin{align*}
            P(x):&\ (x \in \mathbb{R}) \land (x \neq 0)\\
            Q(x):&\ \exists y \in \mathbb{R} \text{ s.t. } xy = 1
        \end{align*}
        then the given statement is $\forall x, (P(x) \implies Q(x))$ as required.

        \item $\exists x \text{ s.t. } (x \in \mathbb{R}) \land (x \neq 0) \land (\forall y \in \mathbb{R}, xy \neq 1)$
    \end{partquestions}
\end{questions}

\subsection*{Problems}
\begin{questions}
    \item \begin{partquestions}{\alph*}
        \item Statement.
        \item Predicate, since it depends on the value of $n$ for the truth or falsity of the expression.
        \item Statement.
        \item Predicate. Although it is true for all real $x$, the truth or falsity can only be determined when a value of $x$ is substituted.
        \item Statement. This is an existential statement.
        \item Predicate. The truth or falsity can only be determined when a value of $x$ is substituted.
        \item Statement. This is a universal statement.
    \end{partquestions}

    \item \begin{partquestions}{\alph*}
        \item We claim that they are not equivalent.
        \begin{table}[h]
            \centering
            \fontsize{8pt}{11pt}\selectfont
            \begin{tabular}{|l|l|l||l|l||l|l|}
                \hline
                $\boldsymbol{p}$ & $\boldsymbol{q}$ & $\boldsymbol{r}$ & $\boldsymbol{p \implies q}$ & $\boldsymbol{q \implies r}$ & $\boldsymbol{p \implies (q \implies r)}$ & $\boldsymbol{(p \implies q) \implies r}$ \\ \hline
                F & F & F & T & T & T & F \\ \hline
                F & F & T & T & T & T & T \\ \hline
                F & T & F & T & F & T & F \\ \hline
                F & T & T & T & T & T & T \\ \hline
                T & F & F & F & T & T & T \\ \hline
                T & F & T & F & T & T & T \\ \hline
                T & T & F & T & F & F & F \\ \hline
                T & T & T & T & T & T & T \\ \hline
            \end{tabular}
        \end{table}

        We can see from the truth table that if $p$ is false, $q$ is true, and $r$ is false, then $p \implies (q \implies r)$ is true while $(p \implies q) \implies r$ is false. Thus $(p \implies (q \implies r)) \not\equiv ((p \implies q) \implies r)$.

        \item We claim that they are equivalent.
        \begin{table}[H]
            \centering
            \fontsize{7.5pt}{11pt}\selectfont
            \begin{tabular}{|l|l|l||l|l||l|l|}
                \hline
                $\boldsymbol{p}$ & $\boldsymbol{q}$ & $\boldsymbol{r}$ & $\boldsymbol{p \iff q}$ & $\boldsymbol{q \iff r}$ & $\boldsymbol{p \iff (q \iff r)}$ & $\boldsymbol{(p \iff q) \iff r}$ \\ \hline
                F & F & F & T & T & F & F \\ \hline
                F & F & T & T & F & T & T \\ \hline
                F & T & F & F & F & T & T \\ \hline
                F & T & T & F & T & F & F \\ \hline
                T & F & F & F & T & T & T \\ \hline
                T & F & T & F & F & F & F \\ \hline
                T & T & F & T & F & F & F \\ \hline
                T & T & T & T & T & T & T \\ \hline
            \end{tabular}
        \end{table}

        By inspection, $(p \iff (q \iff r)) \equiv ((p \iff q) \iff r)$.
    \end{partquestions}

    \item \begin{partquestions}{\alph*}
        \item False. Let $p$ be a false statement and $q$ be a true statement and the result is clear.
        \item True. Set $q$ to be the same as $p$ and result follows.
        \item False. For any statement $p$, if $p$ is true then set $q$ to be a false statement and set $q$ to be true otherwise.
        \item True. Choose any two true statements and it will be clear.
        \item False. Let $p$ and $q$ be both the same statement and the result is clear.
        \item True. If $p$ is true then let $q$ be a false statement, and if $p$ is false then let $q$ be a true statement.
        \item False. For any statement $p$, set $q$ to be the same as $p$ and result follows.
        \item True. Choose a true and false statement and result is clear.
    \end{partquestions}

    \item Recall from \myref{example-implication-law} that $(x \implies y) \equiv \lnot x \lor y$.
    \begin{align*}
        &\lnot p \land (\lnot p \implies (p \land q))\\
        &\equiv \lnot p \land (\lnot(\lnot p) \lor (p \land q)) & (\text{by } \myref{example-implication-law})\\
        &\equiv \lnot p \land (p \lor (p \land q))\\
        &\equiv \lnot p \land ((p \lor p) \land (p \lor q)) & (\text{Distributivity})\\
        &\equiv \lnot p \land (p \land (p \lor q))\\
        &\equiv (\lnot p \land p) \land (p \lor q) & (\text{Associativity})\\
        &\equiv \textbf{false} \land (p \lor q)\\
        &\equiv \textbf{false}.
    \end{align*}
\end{questions}
