\section{Rings and Encryption}
\subsection*{Exercises}
\begin{questions}
    \item We claim that $x+2$ is its own inverse when $N = 2$ and $p = 4$, since
    \begin{align*}
        (x+2)^2 &= x^2 + 4x + 4\\
        &= x^0 + 4x + 4 & (\text{reduce powers modulo } N = 2)\\
        &= 4x + 5\\
        &= 1. & (\text{reduce coefficients modulo } p = 4)
    \end{align*}

    \item Suppose $f(x) \in \mathcal{L}(k,k)$. Then $f(x)$ has exactly $k$ coefficients of 1 and $k$ coefficients of -1. Therefore, evaluating $f(1)$ yields a result of 0.

    The equivalent requirement for $f(x)$ to have an inverse modulo $p$, say $F_p(x)$, is that $F_p(x)f(x) = 1$ within the ring $\Z_p[x]$. However $f(1) = 0$, meaning that $f(x)$ has a zero in $\Z_p$, while the constant polynomial 1 does not. Therefore, there cannot be a polynomial $F_p(x)$ such that $F_p(x)f(x) = 1$ in $\Z_p[x]$, i.e. $f(x)$ does not have an inverse.

    \item Bob's public key is
    \begin{align*}
        h(x) &= F_{16}g(x)\\
        &= (7x^5 + 5x^4 + 14x^3 + 9x^2 + 12x + 2)(x^4 - x^3 - x + 1)\\
        &= 7x^9 - 2x^8 + 9x^7 - 12x^6 + 5x^5 - 19x^4 + 3x^3 - 3x^2 + 10x + 2\\
        &= 7x^3 - 2x^2 + 9x - 12 + 5x^5 - 19x^4 + 3x^3 - 3x^2 + 10x + 2\\
        &= 5x^5 - 19x^4 + 10x^3 - 5x^2 + 19x - 10\\
        &\equiv 5x^5 + 13x^4 + 10x^3 + 11x^2 + 3x + 6. \pmod{16}
    \end{align*}

    \item $x^6 + x^4 + x^2 + 1$

    \item For this case, $\phi(x) = x - 1$ and $m(x) = x^6 + x^4 + x^2 + 1$. Thus
    \begin{align*}
        e(x) &= 3\phi(x)h(x) + m(x) \\
        &= 3(x-1)(24x^7 + 15x^6 + 50x^5 + 48x^4 + 40x^3 + 46x^2\\
        &\quad\quad+ 14x + 19) + (x^6 + x^4 + x^2 + 1)\\
        &= 72x^8 - 27x^7 + 106x^6 - 6x^5 - 23x^4 + 18x^3 - 95x^2\\
        &\quad\quad+ 15x - 56\\
        &= 72 - 27x^7 + 106x^6 - 6x^5 - 23x^4 + 18x^3 - 95x^2\\
        &\quad\quad+ 15x - 56\\
        &= -27x^7 + 106x^6 - 6x^5 - 23x^4 + 18x^3 - 95x^2\\
        &\quad\quad+ 15x + 16\\
        &\equiv 37x^7 + 42x^6 + 58x^5 + 41x^4 + 18x^3 + 33x^2\\
        &\quad\quad+ 15x + 16 \pmod{64}
    \end{align*}
    which means the encrypted message polynomial is $37x^7 + 42x^6 + 58x^5 + 41x^4 + 18x^3 + 33x^2 + 15x + 16$.

    \item We first compute $a(x)$,
    \begin{align*}
        a(x) &= f(x)e(x)\\
        &= (x^7 +x^6 +x^5 -x^4 -x^3 -x + 1)(8x^7 + 12x^6 + 52x^5\\
        &\quad\quad+ 26x^4 +x^3 + 62x^2 + 4x + 29)\\
        &= 8x^{14} + 20x^{13} + 72x^{12} + 82x^{11} + 59x^{10} + 25x^9 - 19x^8\\
        &\quad\quad+ 64x^7 - 70x^6 - 11x^5 - 8x^4 - 90x^3 + 58x^2 - 25x + 29\\
        &= 8x^6 + 20x^5 + 72x^4 + 82x^3 + 59x^2 + 25x - 19 + 64x^7\\
        &\quad\quad- 70x^6 - 11x^5 - 8x^4 - 90x^3 + 58x^2 - 25x + 29\\
        &= 64x^7 - 62x^6 + 9x^5 + 64x^4 - 8x^3 + 117x^2 + 10\\
        &\equiv 2x^6 + 9x^5 - 8x^3 - 11x^2 + 10, \pmod{64}
    \end{align*}
    remembering that we choose coefficients of $a(x)$ to be between -32 and 32. Then we compute $b(x)$ by reducing the coefficients of $a(x)$ modulo 3,
    \[
        b(x) \equiv -x^6 + x^3 + x^2 + 1, \pmod{3}
    \]
    remembering that we choose coefficients of $b(x)$ to be between -1 and 1. Finally we retrieve the original message polynomial,
    \begin{align*}
        F_3(x)b(x) &= (2x^6 +x^5 +x^4 + 2x^2 + 2x + 2)(-x^6 + x^3 + x^2 + 1)\\
        &= -2x^{12} - x^{11} - x^{10} + 2x^9 + x^8 + x^6 + 3x^5 + 5x^4\\
        &\quad\quad+ 4x^3 + 4x^2 + 2x + 2\\
        &= -2x^4 - x^3 - x^2 + 2x + 1 + x^6 + 3x^5 + 5x^4 + 4x^3\\
        &\quad\quad+ 4x^2 + 2x + 2\\
        &= x^6 + 3x^5 + 3x^4 + 3x^3 + 3x^2 + 4x + 3\\
        &\equiv x^6 + x, \pmod{3}
    \end{align*}
    which is the character `B' encoded using \myref{table-ASCII-conversion-table}.
\end{questions}

\subsection*{Problems}
No problems.
